AutoKchp/ReindexNFA.lean
@@ -1,0 +1,698 @@
+/-
+Copyright (c) 2026 Marc Perlade. All rights reserved.
+Released under Apache 2.0 license as described in the file LICENSE.
+Authors: Marc Perlade
+-/
+
+module
+
+public import AutoKchp.NFA
+import Std.Data.HashMap
+import AutoKchp.Internal.Util
+import AutoKchp.Internal.Counting
+
+
+structure DFSState {a: Nat} (r: NFA a) where
+  idx: Std.HashMap r.σ Nat
+  del: Array (Vector (Array Nat) a)
+  fin: Array Bool
+
+
+def reindexFrom {a: Nat} (r: NFA a) (p: r.σ) (s: DFSState r):
+    Nat → DFSState r × Nat
+  | 0 => (s, 0)
+  | fuel + 1 => match s.idx[p]? with
+    | none => let i := s.del.size
+        (
+          Fin.foldl a (fun s b =>
+            (r.δ p b).foldl (
+                fun s q =>
+                    let (s, j) := reindexFrom r q s fuel
+                    { s with del := s.del.modify i (fun v => v.modify b (fun arr => arr.push j))}
+            ) s
+          )
+          {
+            idx := s.idx.insert p i
+            del := s.del.push (Vector.replicate a #[])
+            fin := s.fin.push (r.f p)
+          },
+          i
+        )
+    | some i => (s, i)
+
+
+theorem reindexFrom_preserves {a: Nat} {r: NFA a} {p: r.σ} {s: DFSState r}
+  {u: r.σ} {i: Nat} (h: s.idx[u]? = some i):
+    {fuel: Nat} → (reindexFrom r p s fuel).fst.idx[u]? = some i
+  | 0 => h
+  | _ + 1 => match eq: s.idx[p]? with
+    | none => reindexFrom.eq_def r p s _ ▸ eq ▸
+        Fin.foldl_induction (fun (w: DFSState r) _ => w.idx[u]? = some i)
+          (have ne: p ≠ u := fun eq2 => Option.some_ne_none i (h.symm.trans (eq2 ▸ eq));
+            (Std.HashMap.getElem?_insert_of_ne ne).trans h)
+          (fun _ _ hrec => Array.foldl_induction (fun _ (w: DFSState r) => w.idx[u]? = some i)
+            hrec (fun _ _ hrec => reindexFrom_preserves hrec))
+    | some _ => reindexFrom.eq_def r p s _ ▸ eq ▸ h
+
+
+theorem reindexFrom_preserves2 {a: Nat} {r: NFA a} {p: r.σ} {s: DFSState r}
+  {i: Nat} {v: Vector (Array Nat) a} (h: s.del[i]? = some v):
+    {fuel: Nat} → (reindexFrom r p s fuel).fst.del[i]? = some v
+  | 0 => h
+  | _ + 1 => match eq: s.idx[p]? with
+    | none => reindexFrom.eq_def r p s _ ▸ eq ▸
+      have ⟨lt, eq⟩ := Array.getElem?_eq_some_iff.mp h;
+      Fin.foldl_induction (fun (w: DFSState r) _ => w.del[i]? = some v)
+        ((Array.getElem?_push_lt lt).trans (congrArg some eq))
+        (fun _ _ hrec => Array.foldl_induction (fun _ (w: DFSState r) => w.del[i]? = some v)
+            hrec (fun _ _ hrec => (Array.getElem?_modify.trans (if_neg (Ne.symm (Nat.ne_of_lt lt)))).trans
+                (reindexFrom_preserves2 hrec))
+        )
+    | some _ => reindexFrom.eq_def r p s _ ▸ eq ▸ h
+
+
+theorem reindexFrom_preserves3 {a: Nat} {r: NFA a} {p: r.σ} {s: DFSState r}
+  {i: Nat} {v: Bool} (h: s.fin[i]? = some v):
+    {fuel: Nat} → (reindexFrom r p s fuel).fst.fin[i]? = some v
+  | 0 => h
+  | _ + 1 => match eq: s.idx[p]? with
+    | none => reindexFrom.eq_def r p s _ ▸ eq ▸
+      have ⟨lt, eq⟩ := Array.getElem?_eq_some_iff.mp h;
+      Fin.foldl_induction (fun (w: DFSState r) _ => w.fin[i]? = some v)
+        ((Array.getElem?_push_lt lt).trans (congrArg some eq))
+        (fun _ _ hrec => Array.foldl_induction (fun _ (w: DFSState r) => w.fin[i]? = some v)
+            hrec (fun _ _ hrec => reindexFrom_preserves3 hrec))
+    | some _ => reindexFrom.eq_def r p s _ ▸ eq ▸ h
+
+
+theorem reindexFrom_step {a: Nat} {r: NFA a} {p: r.σ} {s: DFSState r}:
+    {fuel: Nat} → fuel > FiniteHashable.cardinal r.σ - s.idx.size →
+      (reindexFrom r p s fuel).fst.idx[p]? = some (reindexFrom r p s fuel).snd
+  | 0 => fun hf => False.elim (Nat.not_lt_zero _ hf)
+  | _ + 1 => match eq: s.idx[p]? with
+    | none => fun _ => reindexFrom.eq_def r p s _ ▸ eq ▸
+        Fin.foldl_induction (fun (w: DFSState r) _ => w.idx[p]? = some s.del.size)
+          Std.HashMap.getElem?_insert_self
+          (fun _ _ hrec => Array.foldl_induction (fun _ (w: DFSState r) => w.idx[p]? = some s.del.size)
+            hrec (fun _ _ hrec => reindexFrom_preserves hrec))
+    | some _ => fun _ => reindexFrom.eq_def r p s _ ▸ eq ▸ eq
+
+
+theorem reindexFrom_size {a: Nat} {r: NFA a} {p: r.σ} {s: DFSState r}:
+    {fuel: Nat} → (reindexFrom r p s fuel).fst.idx.size ≥ s.idx.size
+  | 0 => Nat.le_refl _
+  | _ + 1 => match eq: s.idx[p]? with
+    | none => reindexFrom.eq_def r p s _ ▸ eq ▸
+        Fin.foldl_induction (fun (w: DFSState r) _ => w.idx.size ≥ s.idx.size)
+          Std.HashMap.size_le_size_insert
+          (fun _ _ hrec => Array.foldl_induction (fun _ (w: DFSState r) => w.idx.size ≥ s.idx.size)
+            hrec (fun _ _ hrec => Nat.le_trans hrec reindexFrom_size))
+    | some _ => reindexFrom.eq_def r p s _ ▸ eq ▸ Nat.le_refl _
+
+
+def invariant {a: Nat} (r: NFA a) (grey: List r.σ) (s: DFSState r): Prop :=
+  s.idx.size = s.del.size ∧ s.idx.size = s.fin.size ∧
+  (∀ i: Nat, i < s.idx.size ↔ (∃ p: r.σ, s.idx[p]? = some i)) ∧
+  (∀ p: r.σ, p ∉ grey → s.idx[p]?.allP
+    (fun i => ∃ hi1: i < s.del.size, ∃ hi2: i < s.fin.size,
+      (∀ b: Fin a, ∃ hs: (s.del[i].get b).size = (r.δ p b).size,
+        ∀ k: Nat, (hk: k < (r.δ p b).size) → s.idx[(r.δ p b)[k]]? = some (s.del[i].get b)[k]) ∧
+      r.f p = s.fin[i]
+    )
+  )
+
+
+def mainMotive {a: Nat} {r: NFA a} (p: r.σ) (grey: List r.σ) (s: DFSState r) (fuel: Nat)
+    (s2: DFSState r) (c: Nat): Prop :=
+  invariant r (p::grey) s2 ∧
+  s2.idx[p]? = some s.del.size ∧
+  (∃ hi1: s.del.size < s2.del.size, ∃ hi2: s.del.size < s2.fin.size,
+    (∀ b: Fin a, b < c →
+      (∃ hs: (s2.del[s.del.size].get b).size = (r.δ p b).size,
+        ∀ k: Nat, (hk: k < (r.δ p b).size) → s2.idx[(r.δ p b)[k]]? = some (s2.del[s.del.size].get b)[k])) ∧
+    (∀ b: Fin a, b ≥ c → s2.del[s.del.size].get b = #[]) ∧
+    r.f p = s2.fin[s.del.size]
+  ) ∧
+  fuel > FiniteHashable.cardinal r.σ - s2.idx.size
+
+
+def subMotive {a: Nat} {r: NFA a} (p: r.σ) (grey: List r.σ) (s: DFSState r) (fuel: Nat) (c: Fin a)
+    (l: Nat) (s2: DFSState r): Prop :=
+  invariant r (p::grey) s2 ∧
+  s2.idx[p]? = some s.del.size ∧
+  (∃ hi1: s.del.size < s2.del.size, ∃ hi2: s.del.size < s2.fin.size,
+    (∀ b: Fin a, b < c → ∃ hs: (s2.del[s.del.size].get b).size = (r.δ p b).size,
+      ∀ k: Nat, (hk: k < (r.δ p b).size) → s2.idx[(r.δ p b)[k]]? = some (s2.del[s.del.size].get b)[k]) ∧
+    (∃ hs: (s2.del[s.del.size].get c).size = l ∧ l ≤ (r.δ p c).size,
+      ∀ k: Nat, (hk: k < l) → s2.idx[(r.δ p c)[k]]? = some (s2.del[s.del.size].get c)[k]) ∧
+    (∀ b: Fin a, b ≥ c.val + 1 → s2.del[s.del.size].get b = #[]) ∧
+    r.f p = s2.fin[s.del.size]
+  ) ∧
+  fuel > FiniteHashable.cardinal r.σ - s2.idx.size
+
+
+def reindexFrom_motive (fuel: Nat): Prop :=
+  {a: Nat} → {r: NFA a} → {p: r.σ} → {s: DFSState r} → (grey: List r.σ) →
+  invariant r grey s → fuel > FiniteHashable.cardinal r.σ - s.idx.size →
+  invariant r grey (reindexFrom r p s fuel).fst
+
+
+theorem subMotive_step {a: Nat} {r: NFA a} {p: r.σ} {grey: List r.σ} {s: DFSState r} {fuel: Nat}
+  {s2: DFSState r} {c: Fin a} {l: Fin (r.δ p c).size} (h: subMotive p grey s fuel c l s2)
+  (hfx: reindexFrom_motive fuel):
+    subMotive p grey s fuel c l.succ
+    {
+      (reindexFrom r (r.δ p c)[l] s2 fuel).fst
+      with del :=
+        (reindexFrom r (r.δ p c)[l] s2 fuel).fst.del.modify s.del.size fun v =>
+          v.modify c fun arr => arr.push (reindexFrom r (r.δ p c)[l] s2 fuel).snd
+    } :=
+  let sr: DFSState r := (reindexFrom r (r.δ p c)[l] s2 fuel).fst
+  have hinv: invariant r (p::grey) sr := hfx (p::grey)
+    h.left h.right.right.right
+  let sr2 := {
+    sr with
+    del := sr.del.modify s.del.size fun v =>
+        v.modify c fun arr => arr.push (reindexFrom r (r.δ p c)[l] s2 fuel).snd,
+  }
+  have concl: subMotive p grey s fuel c l.succ sr2 := ⟨
+    ⟨
+      hinv.left.trans Array.size_modify.symm,
+      hinv.right.left,
+      hinv.right.right.left,
+      fun p2 hp2 =>
+        have ne: sr.idx[p2]? ≠ some s.del.size := fun eq2 =>
+          have ⟨mem, eqp⟩ := Std.HashMap.getElem?_eq_some_iff.mp
+            (reindexFrom_preserves h.right.left)
+          have ⟨mem2, eqp2⟩ := Std.HashMap.getElem?_eq_some_iff.mp eq2
+          have eq3: p2 = p := hashmap_counting_inj hinv.right.right.left
+            p2 p mem2 mem (eqp2.trans eqp.symm)
+          hp2 (eq3 ▸ List.mem_cons_self)
+        have ne2: sr.idx[p2]?.allP (· ≠ s.del.size) := match eq3: sr.idx[p2]? with
+          | some i => (fun eq2 => ne (eq2 ▸ eq3))
+          | none => True.intro
+        Option.allP_mp (Option.allP_and.mp ⟨hinv.right.right.right p2 hp2, ne2⟩)
+          (fun i ⟨⟨hi1, hi2, hi3⟩, hi4⟩ =>
+            have hi1' := Nat.lt_of_lt_of_eq hi1 Array.size_modify.symm
+            ⟨hi1', hi2,
+              ⟨fun b => have ⟨hs, hc⟩ := hi3.left b
+                ⟨Array.getElem_modify_of_ne (Ne.symm hi4) _ hi1' ▸ hs,
+                  fun k hk =>
+                    have hck := hc k hk
+                    hck.trans (congrArg some (getElem_congr_coll
+                      (Array.getElem_modify_of_ne (Ne.symm hi4) _ hi1' ▸ rfl)))
+                ⟩,
+                hi3.right
+              ⟩
+            ⟩
+          ),
+    ⟩,
+    reindexFrom_preserves h.right.left,
+    have ⟨hi1, hi2, hc, hce, hc2, hf⟩ := h.right.right.left
+    have sle: s2.idx.size ≤ sr.idx.size := reindexFrom_size
+    have sle2: s2.del.size ≤ sr.del.size := h.left.left ▸ hinv.left ▸ sle
+    have hi1' := Nat.lt_of_lt_of_le hi1 (Nat.le_trans sle2 (Nat.le_of_eq Array.size_modify.symm))
+    ⟨
+      hi1',
+      Nat.lt_of_lt_of_le hi2 (h.left.right.left ▸ hinv.right.left ▸ sle),
+      fun b hb =>
+        have c: sr.del[s.del.size]? = some s2.del[s.del.size] :=
+          reindexFrom_preserves2 (Array.getElem?_eq_getElem _)
+        have ⟨_, c2⟩ := Array.getElem?_eq_some_iff.mp c
+        have ⟨hs, hs2⟩ := hc b hb
+        have eq: sr2.del[s.del.size].get b = sr.del[s.del.size].get b :=
+          Array.getElem_modify_self _ hi1' ▸
+            Vector.get_modify_of_ne (Fin.ne_of_val_ne (Ne.symm (Nat.ne_of_lt hb)))
+        have eq2: sr2.del[s.del.size].get b = s2.del[s.del.size].get b := c2 ▸ eq
+        ⟨eq2 ▸ hs, fun k hk =>
+          reindexFrom_preserves (((hs2 k hk).trans (congrArg some (getElem_congr_coll eq2).symm)))
+        ⟩,
+      have c1: sr.del[s.del.size]? = some s2.del[s.del.size] :=
+        reindexFrom_preserves2 (Array.getElem?_eq_getElem _)
+      have ⟨_, c2⟩ := Array.getElem?_eq_some_iff.mp c1
+      have eq: sr2.del[s.del.size].get c = (s2.del[s.del.size].get c).push
+          (reindexFrom r (r.δ p c)[l] s2 fuel).snd :=
+        (congrArg (fun (w: Vector _ a) => w.get c) (Array.getElem_modify_self _ hi1')).trans (
+          Vector.get_modify_self.trans (congrArg (fun (w: Vector (Array _) a) => (w.get c).push _) c2))
+      have ⟨⟨heq, hle⟩, hh⟩ := hce
+      ⟨⟨eq ▸ (heq ▸ Array.size_push _), Nat.succ_le_of_lt l.isLt⟩, fun k hk =>
+        (Eq.trans (
+          match Nat.lt_or_eq_of_le (Nat.le_of_lt_succ hk) with
+          | .inl lt => reindexFrom_preserves (Array.getElem_push_lt (heq ▸ lt) ▸ hh k lt)
+          | .inr eq2 =>
+            have eq3: (r.δ p c)[k] = (r.δ p c)[l] := getElem_congr_idx eq2
+            Eq.trans (eq3.substr (reindexFrom_step h.right.right.right))
+              (congrArg some ((getElem_congr_idx (eq2.trans heq.symm)).trans Array.getElem_push_eq)).symm
+        ) (congrArg some (getElem_congr_coll (i := k) eq)).symm)
+      ⟩,
+      fun b hb =>
+        have c: sr.del[s.del.size]? = some s2.del[s.del.size] :=
+          reindexFrom_preserves2 (Array.getElem?_eq_getElem _)
+        have ⟨_, c2⟩ := Array.getElem?_eq_some_iff.mp c
+        Array.getElem_modify_self _ hi1' ▸
+          (Vector.get_modify_of_ne (Fin.ne_of_val_ne (Nat.ne_of_lt (Nat.lt_of_succ_le hb)))).symm ▸
+          c2 ▸ (hc2 b hb),
+      have c: sr.fin[s.del.size]? = some (r.f p) :=
+        reindexFrom_preserves3 (Array.getElem?_eq_getElem hi2 ▸ congrArg some hf.symm)
+      have ⟨_, c2⟩ := Array.getElem?_eq_some_iff.mp c
+      c2.symm
+    ⟩,
+    Nat.lt_of_le_of_lt (Nat.sub_le_sub_left reindexFrom_size _) h.right.right.right,
+  ⟩
+  concl
+
+
+theorem mainMotive_step {a: Nat} {r: NFA a} {p: r.σ} {grey: List r.σ} {s: DFSState r} {fuel: Nat}
+  {s2: DFSState r} {c: Fin a} (h: mainMotive p grey s fuel s2 c)
+  (hfx: reindexFrom_motive fuel): mainMotive p grey s fuel
+    ((r.δ p c).foldl
+      (fun s2 q => {
+        (reindexFrom r q s2 fuel).fst
+        with del :=
+          (reindexFrom r q s2 fuel).fst.del.modify s.del.size fun v =>
+            v.modify c fun arr => arr.push (reindexFrom r q s2 fuel).snd
+      })
+    s2)
+    c.val.succ :=
+  let sf2: DFSState r := (r.δ p c).foldl
+      (fun s2 q => {
+        (reindexFrom r q s2 fuel).fst
+        with del :=
+          (reindexFrom r q s2 fuel).fst.del.modify s.del.size fun v =>
+            v.modify c fun arr => arr.push (reindexFrom r q s2 fuel).snd
+      })
+    s2
+  have ind2: subMotive p grey s fuel c (r.δ p c).size sf2 := Array.foldl_induction
+    (subMotive p grey s fuel c)
+    ⟨
+      h.left,
+      h.right.left,
+      have ⟨hi1, hi2, hc, hc2, hf⟩ := h.right.right.left
+      ⟨
+        hi1, hi2, hc,
+        ⟨⟨Array.size_eq_zero_iff.mpr (hc2 c (Nat.le_refl c)), Nat.zero_le _⟩,
+          fun k hk => False.elim (Nat.not_lt_zero k hk)⟩,
+        fun b hb => hc2 b (Nat.le_of_succ_le hb),
+        hf
+      ⟩,
+      h.right.right.right,
+    ⟩
+    (fun l s2 hrec => subMotive_step hrec hfx)
+  ⟨
+    ind2.left,
+    ind2.right.left,
+    have ⟨hi1, hi2, hcl, ⟨hs, hce⟩, hcl2, hf⟩ := ind2.right.right.left
+    ⟨
+      hi1, hi2,
+      fun b hb => match Nat.lt_or_eq_of_le (Nat.le_of_lt_succ hb) with
+      | .inl lt => hcl b lt
+      | .inr eq => have eq := Fin.eq_of_val_eq eq
+        ⟨eq.symm ▸ hs.left, eq.symm ▸ hce⟩,
+      hcl2, hf,
+    ⟩,
+    ind2.right.right.right
+  ⟩
+
+
+theorem reindexFrom_correct {a: Nat} {r: NFA a} {p: r.σ}
+  {s: DFSState r} (grey: List r.σ) (h: invariant r grey s):
+    {fuel: Nat} → fuel > FiniteHashable.cardinal r.σ - s.idx.size →
+      invariant r grey (reindexFrom r p s fuel).fst
+  | 0 => fun _ => h
+  | fuel + 1 => match eq: s.idx[p]? with
+    | none => fun hf =>
+      let sf: DFSState r := Fin.foldl a
+        (fun s2 b =>
+           (r.δ p b).foldl
+            (fun s2 q => {
+                idx := (reindexFrom r q s2 fuel).fst.idx,
+                del :=
+                  (reindexFrom r q s2 fuel).fst.del.modify s.del.size fun v =>
+                    v.modify b fun arr => arr.push (reindexFrom r q s2 fuel).snd,
+                fin := (reindexFrom r q s2 fuel).fst.fin
+              }
+            ) s2
+        )
+        {
+          idx := s.idx.insert p s.del.size
+          del := s.del.push (Vector.replicate a #[])
+          fin := s.fin.push (r.f p)
+        }
+      have concl: invariant r grey sf := (
+        have ind: mainMotive p grey s fuel sf a := Fin.foldl_induction (mainMotive p grey s fuel)
+          --Initialization
+          ⟨
+            have hidx: (s.idx.insert p s.del.size).size = s.idx.size + 1 :=
+              Std.HashMap.size_insert.trans (dif_neg (Std.HashMap.getElem?_eq_none_iff.mp eq))
+            ⟨
+              (hidx.trans (congrArg (· + 1) h.left)).trans (Array.size_push _).symm,
+              (hidx.trans (congrArg (· + 1) h.right.left)).trans (Array.size_push _).symm,
+              fun i =>
+                have hi0 := h.right.right.left i
+                hidx ▸ ⟨
+                  fun hi => match Nat.lt_or_eq_of_le (Nat.le_of_lt_succ hi) with
+                    | .inl lt => have ⟨p2, hp2⟩ := hi0.mp lt
+                      ⟨p2, (Std.HashMap.getElem?_insert_of_ne (
+                        fun eq2 => Option.some_ne_none _ ((eq2 ▸ hp2).symm.trans eq)
+                      )).trans hp2⟩
+                    | .inr eq2 => ⟨p, (eq2.trans h.left) ▸ Std.HashMap.getElem?_insert_self⟩,
+                  fun ⟨p2, hp2⟩ =>
+                    if eq2: p = p2 then
+                      have is: (s.idx.insert p s.del.size)[p2]? = some s.del.size :=
+                        eq2 ▸ Std.HashMap.getElem?_insert_self
+                      (Option.some_inj.mp (h.left ▸ is.symm.trans hp2)) ▸ Nat.lt_succ_self s.idx.size
+                    else
+                      Nat.lt_succ_of_lt (hi0.mpr ⟨p2,
+                        (Std.HashMap.getElem?_insert_of_ne eq2).symm.trans hp2⟩),
+                ⟩,
+              fun p2 nmem =>
+                (Std.HashMap.getElem?_insert_of_ne (fun eq2 => nmem (eq2.subst List.mem_cons_self))).symm ▸
+                Option.allP_mp (h.right.right.right p2 (mt (List.mem_cons_of_mem p) nmem)) (
+                  fun i ⟨hi1, hi2, hc, hf⟩ => ⟨
+                    Array.size_push _ ▸ Nat.lt_succ_of_lt hi1,
+                    Array.size_push _ ▸ Nat.lt_succ_of_lt hi2,
+                    fun b => have ⟨hs, hcb⟩ := hc b
+                      ⟨
+                        (Array.getElem_push_lt hi1) ▸ hs,
+                        fun k hk =>
+                          have hck := hcb k hk
+                          have ne: p ≠ (r.δ p2 b)[k] :=
+                            fun eq2 => Option.some_ne_none _ ((eq2 ▸ hck).symm.trans eq)
+                          (Std.HashMap.getElem?_insert_of_ne ne).trans (hck.trans
+                            (congrArg some (getElem_congr_coll (congrArg
+                              (fun (w: Vector _ a) => w.get b) (Array.getElem_push_lt hi1).symm))))
+                      ⟩,
+                    hf.trans (Array.getElem_push_lt hi2).symm,
+                  ⟩
+                )
+            ⟩,
+            Std.HashMap.getElem?_insert_self,
+            have hsz := h.right.left.symm.trans h.left
+            ⟨
+              Array.size_push _ ▸ Nat.lt_succ_self _,
+              hsz ▸ Array.size_push _ ▸ Nat.lt_succ_self _,
+              fun b hb => False.elim (Nat.not_lt_zero b hb),
+              fun b _ => Array.getElem_push_eq ▸ Vector.get_replicate,
+              Array.getElem_push_eq.symm.trans (getElem_congr_idx hsz),
+            ⟩,
+            Nat.lt_of_lt_of_le (FiniteHashable.hashmap_insert_remaining_lt
+              (fun mem => nomatch (eq ▸ Std.HashMap.isSome_getElem?_iff_mem.mpr mem)))
+              (Nat.le_of_lt_succ hf),
+          ⟩
+          --Induction
+          (fun s2 c hrec => mainMotive_step hrec (fun grey h1 h2 => reindexFrom_correct grey h1 h2))
+        ⟨
+          ind.left.left,
+          ind.left.right.left,
+          ind.left.right.right.left,
+          fun p2 hp2 => if eq2: p = p2 then
+            have ⟨hi1, hi2, hc, _, hf⟩ := ind.right.right.left
+            (eq2 ▸ ind.right.left) ▸ ⟨hi1, hi2, fun b => eq2 ▸ hc b b.isLt, eq2 ▸ hf⟩
+          else
+            ind.left.right.right.right p2 (fun mem => match List.mem_cons.mp mem with
+              | .inl eq3 => eq2 eq3.symm | .inr mem2 => hp2 mem2),
+        ⟩
+      )
+      reindexFrom.eq_def r p s _ ▸ eq ▸ concl
+    | some _ => fun _ => reindexFrom.eq_def r p s _ ▸ eq ▸ h
+
+
+def reindex {a: Nat} (r: NFA a): DFSState r × Array Nat :=
+  r.i.foldl (fun (s, init) p =>
+    let (s, i) := reindexFrom r p s (FiniteHashable.cardinal r.σ + 1)
+    (s, init.push i)
+  ) ({ idx := ∅, del := #[], fin := #[] }, #[])
+
+
+def reindexCorrectness {a: Nat} {r: NFA a} (s: DFSState r): Prop :=
+  s.idx.size = s.del.size ∧ s.idx.size = s.fin.size ∧
+  (∀ i: Nat, i < s.idx.size ↔ (∃ p: r.σ, s.idx[p]? = some i)) ∧
+  (∀ p: r.σ, s.idx[p]?.allP
+    (fun i => ∃ hi1: i < s.del.size, ∃ hi2: i < s.fin.size,
+      (∀ b: Fin a, ∃ hs: (s.del[i].get b).size = (r.δ p b).size,
+        ∀ k: Nat, (hk: k < (r.δ p b).size) → s.idx[(r.δ p b)[k]]? = some (s.del[i].get b)[k]) ∧
+      r.f p = s.fin[i]
+    )
+  )
+
+
+theorem reindex_correct {a: Nat} {r: NFA a}:
+    reindexCorrectness (reindex r).fst :=
+  have concl: invariant r [] (reindex r).fst := Array.foldl_induction
+    (fun _ (w: DFSState r × Array Nat) => invariant r [] w.fst)
+    ⟨
+      Std.HashMap.size_empty, Std.HashMap.size_empty,
+      (fun i => ⟨
+        fun lt => False.elim (Nat.not_lt_zero i (Std.HashMap.size_empty ▸ lt)),
+        fun ⟨_, hp⟩ => nomatch (Std.HashMap.getElem?_empty ▸ hp)
+      ⟩),
+      fun _ _ => Std.HashMap.getElem?_empty ▸ True.intro
+    ⟩
+    (fun _ _ hrec => reindexFrom_correct [] hrec (Nat.lt_succ_of_le (Nat.sub_le _ _)))
+  ⟨concl.left, concl.right.left, concl.right.right.left,
+    fun p => concl.right.right.right p List.not_mem_nil⟩
+
+
+theorem reindex_start_correct {a: Nat} {r: NFA a}:
+    ∃ hs: (reindex r).snd.size = r.i.size,
+    ∀ k: Nat, (hk: k < r.i.size) → (reindex r).fst.idx[r.i[k]]? = some (reindex r).snd[k] :=
+  let motive (l: Nat) (res: DFSState r × Array Nat): Prop :=
+    ∃ hs: res.snd.size = l ∧ l ≤ r.i.size,
+    ∀ k: Nat, (hk: k < l) → res.fst.idx[r.i[k]]? = some res.snd[k]
+  have ⟨⟨hs1, _⟩, c⟩: motive r.i.size (reindex r) := Array.foldl_induction motive
+    ⟨⟨rfl, Nat.zero_le _⟩, fun k hk => False.elim (Nat.not_lt_zero k hk)⟩
+    (fun l res ⟨⟨hs1, hs2⟩, hrec⟩ =>
+      ⟨⟨hs1 ▸ Array.size_push _, Nat.succ_le_of_lt l.isLt⟩, fun k hk =>
+        match Nat.lt_or_eq_of_le (Nat.le_of_lt_succ hk) with
+        | .inl lt => Array.getElem_push_lt (hs1 ▸ lt) ▸ reindexFrom_preserves (hrec k lt)
+        | .inr eq =>
+          have eq2: r.i[k] = r.i[l] := getElem_congr_idx eq
+          Eq.trans (eq2 ▸ reindexFrom_step (Nat.lt_succ_of_le (Nat.sub_le _ _))) (congrArg some
+            ((getElem_congr_idx (eq.trans hs1.symm)).trans Array.getElem_push_eq).symm)
+      ⟩
+    )
+  ⟨hs1, c⟩
+
+
+def constructReindexed {a: Nat} (r: NFA a): NatNFA a :=
+  let res := reindex r
+  let s := res.fst
+  have hs: reindexCorrectness s := reindex_correct
+  let del: Array (Vector (Array (Fin s.idx.size)) a) :=
+    s.del.pmap (fun v hv => v.pmap (fun v2 hv2 => v2.pmap (fun i hi => ⟨i,
+      have ⟨j, hj1, hj2⟩ := Array.getElem_of_mem hv
+      have ⟨p, hp⟩ := (hs.right.right.left j).mp (hs.left ▸ hj1)
+      have ⟨hj3, hj4, hj5⟩ := hp ▸ hs.right.right.right p
+      have ⟨b, hb⟩ := Vector.get_of_mem hv2
+      have ⟨k, hk1, hk2⟩ := Array.getElem_of_mem hi
+      have ⟨hs2, hj6⟩ := hj5.left b
+      have eq := hj2 ▸ hb
+      have lt: k < (r.δ p b).size := hs2 ▸ eq ▸ hk1
+      (hs.right.right.left i).mpr ⟨(r.δ p b)[k], (hj6 k lt).trans
+        (congrArg some ((getElem_congr_coll eq).trans hk2))⟩
+    ⟩) (fun _ => id)) (fun _ => id)) (fun _ => id)
+  {
+    n := s.idx.size,
+    i := res.snd.attach.map (fun ⟨i, hi⟩ => ⟨i,
+        have ⟨k, hk1, hk2⟩ := Array.getElem_of_mem hi
+        have ⟨hss, h⟩ := reindex_start_correct (r := r)
+        (hs.right.right.left i).mpr ⟨r.i[k], hk2 ▸ h k (hss ▸ hk1)⟩
+      ⟩),
+    δ := fun j b => (del[j]'(Nat.lt_of_lt_of_eq (hs.left ▸ j.isLt) Array.size_pmap.symm)).get b,
+    f := fun j => s.fin[j]'(hs.right.left ▸ j.isLt)
+  }
+
+
+theorem constructReindex_delta_size {a: Nat} {r: NFA a}
+  {i: Fin (reindex r).fst.idx.size} {b: Fin a}:
+    ((constructReindexed r).δ i b).size =
+      (((reindex r).fst.del[i]'(reindex_correct.left ▸ i.isLt)).get b).size :=
+  (congrArg (fun (w: Vector (Array _) a) => (w.get b).size) (Array.getElem_pmap _ _ _)).trans (
+    (congrArg Array.size (Vector.get_pmap _)).trans Array.size_pmap)
+
+
+theorem constructReindexed_delta {a: Nat} {r: NFA a} {i: Fin (reindex r).fst.idx.size}
+  {b: Fin a} {k: Nat} (hk: k < ((constructReindexed r).δ i b).size):
+    ((constructReindexed r).δ i b)[k].val =
+    (((reindex r).fst.del[i]'(reindex_correct.left ▸ i.isLt)).get b)[k]'
+      (constructReindex_delta_size ▸ hk) :=
+  (congrArg Fin.val (getElem_congr_coll (
+    (congrArg (fun (w: Vector _ a) => w.get b) (Array.getElem_pmap _ _ _)).trans
+    (Vector.get_pmap _)
+  ))).trans ((congrArg Fin.val (Array.getElem_pmap _ _ _)))
+
+
+theorem constructReindexed_delta' {a: Nat} {r: NFA a} {p q: r.σ} (hp: p ∈ (reindex r).fst.idx) {b: Fin a}:
+    q ∈ r.δ p b ↔ ∃ hq: q ∈ (reindex r).fst.idx,
+      ⟨(reindex r).fst.idx[q], (reindex_correct.right.right.left _).mpr
+        ⟨q, Std.HashMap.getElem?_eq_some_getElem _⟩⟩ ∈ (constructReindexed r).δ
+      ⟨(reindex r).fst.idx[p], (reindex_correct.right.right.left _).mpr
+        ⟨p, Std.HashMap.getElem?_eq_some_getElem _⟩⟩ b :=
+  have eqp := Std.HashMap.getElem?_eq_some_getElem hp
+  have ⟨hi1, hi2, hi3, _⟩ := eqp ▸ reindex_correct.right.right.right p
+  have ⟨hs, h2⟩ := hi3 b
+  let i: Fin (reindex r).fst.idx.size := ⟨(reindex r).fst.idx[p], reindex_correct.left ▸  hi1⟩
+  have hs2: ((constructReindexed r).δ i b).size =
+    ((reindex r).fst.del[i].get b).size := constructReindex_delta_size
+  have hs3 := hs2.trans hs
+  ⟨
+    fun qmem =>
+      have ⟨k, hk1, hk2⟩ := Array.getElem_of_mem qmem
+      have hk3: k < ((constructReindexed r).δ i b).size := hs3 ▸ hk1
+      have ⟨hq, hq2⟩ := Std.HashMap.getElem?_eq_some_iff.mp (hk2 ▸ h2 k hk1)
+      have ddef: (((constructReindexed r).δ i b)[k]'hk3).val = ((reindex r).fst.del[i].get b)[k] :=
+        constructReindexed_delta hk3
+      have eq := hq2.trans ddef.symm
+      have eq2: ((constructReindexed r).δ i b)[k] = ⟨(reindex r).fst.idx[q], _⟩ :=
+        Fin.eq_of_val_eq eq.symm
+      ⟨hq, Array.mem_of_getElem eq2⟩,
+    fun ⟨hq, hq2⟩ =>
+      have ⟨k, hk1, hk2⟩ := Array.getElem_of_mem hq2
+      have hk3: k < (r.δ p b).size := hs3 ▸ hk1
+      have ddef: (((constructReindexed r).δ i b)[k]'hk1).val = ((reindex r).fst.del[i].get b)[k] :=
+        constructReindexed_delta hk1
+      have eq: ((reindex r).fst.del[i].get b)[k] = (reindex r).fst.idx[q] :=
+        ddef.symm.trans (congrArg Fin.val hk2)
+      have ⟨hq3, hq4⟩ := Std.HashMap.getElem?_eq_some_iff.mp (eq ▸ h2 k hk3)
+      have eq2: (r.δ p b)[k] = q := hashmap_counting_inj reindex_correct.right.right.left
+        (r.δ p b)[k] q hq3 hq hq4
+      Array.mem_of_getElem eq2
+  ⟩
+
+
+theorem constructReindexed_path {a: Nat} {r: NFA a} {p q: r.σ} (h: p ∈ r.i) {l: List (Fin a)}:
+    r.path p q l ↔
+    ∃ (hp: p ∈ (reindex r).fst.idx) (hq: q ∈ (reindex r).fst.idx), (constructReindexed r).path
+      ⟨(reindex r).fst.idx[p], (reindex_correct.right.right.left _).mpr
+        ⟨p, Std.HashMap.getElem?_eq_some_getElem _⟩⟩
+      ⟨(reindex r).fst.idx[q], (reindex_correct.right.right.left _).mpr
+        ⟨q, Std.HashMap.getElem?_eq_some_getElem _⟩⟩ l :=
+  match List.eq_nil_or_concat l with
+  | .inl eq =>
+    have ⟨k, hk1, hk2⟩ := Array.getElem_of_mem h
+    have ⟨hs, h2⟩ := reindex_start_correct (r := r)
+    have ⟨hp0, _⟩ := Std.HashMap.getElem?_eq_some_iff.mp (h2 k hk1)
+    have hp: p ∈ (reindex r).fst.idx := hk2 ▸ hp0
+    eq ▸ ⟨
+      fun eq2 => ⟨hp, eq2 ▸ hp, eq2 ▸ rfl⟩,
+      fun ⟨hp, hq, eq2⟩ => hashmap_counting_inj reindex_correct.right.right.left
+        p q hp hq (Fin.val_eq_of_eq eq2)
+    ⟩
+  | .inr ⟨s, b, eq⟩ => eq ▸ List.concat_eq_append ▸ NFA.path_concat.trans ⟨
+    fun ⟨u, hu1, hu2⟩ =>
+      have ⟨hp, hu, h0⟩ := (constructReindexed_path h).mp hu1
+      have ⟨hq, hq2⟩ := (constructReindexed_delta' hu).mp hu2
+      ⟨hp, hq, NatNFA.path_concat.mpr ⟨⟨(reindex r).fst.idx[u], _⟩, h0, hq2⟩⟩,
+    fun ⟨hp, hq, hpq⟩ =>
+      have ⟨j, hj1, hj2⟩ := NatNFA.path_concat.mp hpq
+      have ⟨u, hu⟩ := (reindex_correct.right.right.left j).mp j.isLt
+      have ⟨hu2, hu3⟩ := Std.HashMap.getElem?_eq_some_iff.mp hu
+      have eq: j = ⟨(reindex r).fst.idx[u], hu3 ▸ j.isLt⟩ := Fin.eq_of_val_eq hu3.symm
+      have h0 := (constructReindexed_path h).mpr ⟨hp, hu2, eq ▸ hj1⟩
+      ⟨u, h0, (constructReindexed_delta' hu2).mpr ⟨hq, eq ▸ hj2⟩⟩,
+  ⟩
+  termination_by l.length
+
+
+theorem constructReindexed_initial {a: Nat} {r: NFA a} {p: r.σ}:
+    p ∈ r.i ↔ ∃ hp: p ∈ (reindex r).fst.idx,
+      ⟨(reindex r).fst.idx[p], (reindex_correct.right.right.left _).mpr
+        ⟨p, Std.HashMap.getElem?_eq_some_getElem _⟩⟩ ∈ (constructReindexed r).i :=
+  have ⟨hs, hs2⟩ := reindex_start_correct (r := r)
+  have hs3: (constructReindexed r).i.size = r.i.size :=
+    Array.size_map.trans (Array.size_attach.trans hs)
+  ⟨
+    fun mem =>
+      have ⟨k, hk1, hk2⟩ := Array.getElem_of_mem mem
+      have ⟨hp, hp2⟩ := Std.HashMap.getElem?_eq_some_iff.mp (hk2 ▸ hs2 k hk1)
+      ⟨hp, Array.mem_map.mpr ⟨⟨(reindex r).fst.idx[p], hp2 ▸ Array.getElem_mem _⟩,
+        Array.mem_attach _ _, rfl⟩⟩,
+    fun ⟨hp, mem⟩ =>
+      have ⟨k, hk1, hk2⟩ := Array.getElem_of_mem mem
+      have ⟨hp2, hp3⟩ := Std.HashMap.getElem?_eq_some_iff.mp (hs2 k (hs3 ▸ hk1))
+      have eq: (constructReindexed r).i[k].val = (reindex r).snd[k] :=
+        (congrArg Fin.val (Array.getElem_map _ _)).trans
+        (congrArg Subtype.val (Array.getElem_attach _))
+      have eq2 := hk2 ▸ hp3.trans eq.symm
+      have eq3 := hashmap_counting_inj reindex_correct.right.right.left r.i[k] p hp2 hp eq2
+      Array.mem_of_getElem eq3
+  ⟩
+
+
+theorem constructReindexed_final {a: Nat} {r: NFA a} {p: r.σ} (hp: p ∈ (reindex r).fst.idx):
+    r.f p ↔ (constructReindexed r).f ⟨(reindex r).fst.idx[p], (reindex_correct.right.right.left _).mpr
+      ⟨p, Std.HashMap.getElem?_eq_some_getElem _⟩⟩ :=
+  have hp2 := Std.HashMap.getElem?_eq_some_getElem hp
+  have ⟨_, _, _, hf⟩ := hp2 ▸ reindex_correct.right.right.right p
+  hf ▸ Iff.refl _
+
+
+theorem constructReindexed_successfulPath {a: Nat} {r: NFA a} {p q: r.σ} {l: List (Fin a)}:
+    r.successfulPath p q l ↔ ∃ (hp: p ∈ (reindex r).fst.idx) (hq: q ∈ (reindex r).fst.idx),
+      (constructReindexed r).successfulPath
+      ⟨(reindex r).fst.idx[p], (reindex_correct.right.right.left _).mpr
+        ⟨p, Std.HashMap.getElem?_eq_some_getElem _⟩⟩
+      ⟨(reindex r).fst.idx[q], (reindex_correct.right.right.left _).mpr
+        ⟨q, Std.HashMap.getElem?_eq_some_getElem _⟩⟩ l :=
+  ⟨
+    fun ⟨h, hi, hf⟩ =>
+      have ⟨hp, hq, h2⟩ := (constructReindexed_path hi).mp h
+      have ⟨_, hi2⟩ := constructReindexed_initial.mp hi
+      ⟨hp, hq, h2, hi2, (constructReindexed_final hq).mp hf⟩,
+    fun ⟨hp, hq, h, hi, hf⟩ =>
+      have hi2 := constructReindexed_initial.mpr ⟨hp, hi⟩
+      have h2 := (constructReindexed_path hi2).mpr ⟨hp, hq, h⟩
+      ⟨h2, hi2, (constructReindexed_final hq).mpr hf⟩
+  ⟩
+
+
+theorem constructReindexed_accepts {a: Nat} {r: NFA a} {l: List (Fin a)}:
+    r.accepts l ↔ (constructReindexed r).accepts l :=
+  ⟨
+    fun ⟨p, q, h⟩ => have ⟨_, _, h2⟩ := constructReindexed_successfulPath.mp h; ⟨_, _, h2⟩,
+    fun ⟨p, q, h⟩ =>
+      have ⟨p2, hp2⟩ := (reindex_correct.right.right.left p).mp p.isLt
+      have ⟨q2, hq2⟩ := (reindex_correct.right.right.left q).mp q.isLt
+      have ⟨hp22, eqp2⟩ := Std.HashMap.getElem?_eq_some_iff.mp hp2
+      have ⟨hq22, eqq2⟩ := Std.HashMap.getElem?_eq_some_iff.mp hq2
+      have eqp3: p = ⟨(reindex r).fst.idx[p2], _⟩ := Fin.eq_of_val_eq eqp2.symm
+      have eqq3: q = ⟨(reindex r).fst.idx[q2], _⟩ := Fin.eq_of_val_eq eqq2.symm
+      ⟨p2, q2, constructReindexed_successfulPath.mpr ⟨hp22, hq22, eqp3 ▸ eqq3 ▸ h⟩⟩
+  ⟩
+
+
+theorem constructReindexed_accepts' {a: Nat} {r: NFA a}:
+    (constructReindexed r).accepts = r.accepts :=
+  funext (fun _ => propext constructReindexed_accepts.symm)
+
+
+public section
+namespace NFA
+
+structure ReindexResult {a: Nat} (r: NFA a) where
+  reindexed: NatNFA a
+  correct: reindexed.accepts = r.accepts
+
+
+def reindex {a: Nat} (r: NFA a): ReindexResult r := {
+  reindexed := constructReindexed r
+  correct := constructReindexed_accepts'
+}
+
+end NFA
+
+namespace NatNFA
+
+structure TrimResult {a: Nat} (r: NatNFA a) where
+  trimmed: NatNFA a
+  correct: trimmed.accepts = r.accepts
+
+
+def trim {a: Nat} (r: NatNFA a): TrimResult r := {
+  trimmed := constructReindexed r.toNFA
+  correct := constructReindexed_accepts'.trans
+    (funext fun _ => propext NatNFA.accepts_toNFA)
+}
+
+end NatNFA
+end
